# 
#    Portions Copyright (c) 2009-10 Zepheira LLC, Some Rights Reserved
#    Portions Copyright (c) 2010-11 Talis Inc, Some Rights Reserved
# 
#    Licensed under the Apache License, Version 2.0 (the "License");
#    you may not use this file except in compliance with the License.
#    You may obtain a copy of the License at
# 
#        http://www.apache.org/licenses/LICENSE-2.0
# 
#    Unless required by applicable law or agreed to in writing, software
#    distributed under the License is distributed on an "AS IS" BASIS,
#    WITHOUT WARRANTIES OR CONDITIONS OF ANY KIND, either express or implied.
#    See the License for the specific language governing permissions and
#    limitations under the License.
#
@prefix xsd:<http://www.w3.org/2001/XMLSchema#>.
@prefix rdf:<http://www.w3.org/1999/02/22-rdf-syntax-ns#>.
@prefix rdfs:<http://www.w3.org/2000/01/rdf-schema#>.
@prefix owl:<http://www.w3.org/2002/07/owl#>.
@prefix obj:<http://www.openrdf.org/rdf/2009/object#>.
@prefix http:<http://www.openrdf.org/rdf/2009/httpobject#>.
@prefix calli:<http://callimachusproject.org/rdf/2009/framework#>.

@base <http://callimachusproject.org/rdf/2009/framework>.

################################
# Ontology
################################

<> a owl:Ontology.

################################
# Class
################################

calli:Alias a owl:Class;
	rdfs:comment "".

calli:Copyable a owl:Class;
	rdfs:comment "Resources that can be copied to create new resources.".

calli:Editable a owl:Class;
	rdfs:comment "Resources that can be edited.".

calli:Viewable a owl:Class;
	rdfs:comment "Resources that can be viewed from a Web browser.".

calli:Template a owl:Class;
	rdfs:comment "RDFa template.".

calli:Realm a owl:Class;
	rdfs:comment "A realm.".

calli:AnybodyRealm a owl:Class;
	rdfs:subClassOf calli:Realm;
	rdfs:comment "A realm that authenticates any agent.".

calli:NobodyRealm a owl:Class;
	rdfs:subClassOf calli:Realm;
	rdfs:comment "A realm that forbids all agents.".

calli:LocalRealm a owl:Class;
	rdfs:subClassOf calli:Realm;
	rdfs:comment "A realm that only authenticates local agents.".

calli:DigestRealm a owl:Class;
	rdfs:subClassOf calli:Realm;
	rdfs:comment "A realm that authenticates HTTP digest credentials.".

calli:Credential a owl:Class;
	rdfs:comment "A digest credentials with a MD5 algorithm.";
	rdfs:subClassOf calli:Party.

calli:User a owl:Class;
	rdfs:comment "Credentials for a person.";
	rdfs:subClassOf calli:Credential.

calli:Group a owl:Class;
	rdfs:comment "A collection of credentials.";
	rdfs:subClassOf calli:Party.

calli:Party a owl:Class;
	rdfs:comment "A credential, user or group of credentials.".

calli:NamedGraph a owl:Class;
	rdfs:comment "Graph in the RDF store that can be retrieved remotely.".

calli:ScriptBundle rdfs:subClassOf rdf:Seq;
	rdfs:comment "A collection of JavaScript files that are downloaded and compressed together.".

################################
# Annotation
################################

calli:conservator a owl:AnnotationProperty;
	rdfs:comment "Credential or group of credentials that can maintain individual resources of this class.".

calli:reviewer a owl:AnnotationProperty;
	rdfs:comment "Credential or group of credentials that can view individual resources of this class.".

calli:copy a owl:AnnotationProperty;
	rdfs:comment "The RDFa template used to copy individual resources of this class using a Web browser.".

calli:edit a owl:AnnotationProperty;
	rdfs:comment "The RDFa template used to edit individual resources of this class using a Web browser.".

calli:view a owl:AnnotationProperty;
	rdfs:comment "The RDFa template used to display individual resources of this class in a Web browser.".

################################
# Property
################################

calli:algorithm a owl:DatatypeProperty, owl:FunctionalProperty;
	rdfs:comment "A value of 'MD5' indicates this credential is a digest credential.";
	rdfs:domain calli:Credential;
	rdfs:range xsd:string.

calli:encoded a owl:DatatypeProperty, owl:FunctionalProperty;
	rdfs:comment "The MD5 encoded username:realm:password";
	rdfs:domain calli:Credential;
	rdfs:range xsd:hexBinary.

calli:name a owl:DatatypeProperty, owl:FunctionalProperty;
	rdfs:comment "The username for this credential.";
	rdfs:domain calli:Credential;
	rdfs:range xsd:string.

calli:email a owl:DatatypeProperty, owl:FunctionalProperty;
	rdfs:comment "The primary email address for this user.";
	rdfs:domain calli:User;
	rdfs:range xsd:string.

calli:authenticates a owl:ObjectProperty;
	rdfs:comment "Group of credentials that can be authenticated by this realm.";
	rdfs:domain calli:DigestRealm;
	rdfs:range calli:Group.

calli:authName a rdf:Property, owl:FunctionalProperty;
	rdfs:comment "A string to be displayed to users so they know which username and password to use. This string should contain at least the name of the host performing the authentication and might additionally indicate the collection of users who might have access. This string is used to encode the passwords and changing it will invalidates existing encoded passwords.";
	rdfs:domain calli:DigestRealm.

calli:origin a rdf:Property;
	rdfs:comment "Identifies the security contexts that allow user agent scripts to initiate an HTTP request that can be seamlessly authenticated with this realm. Include '*' to allow all other contexts without agent credentials.";
	rdfs:domain calli:Realm.

calli:domain a rdf:Property;
	rdfs:comment "Define the protection space for this realm to authenticate. Any URI that has a URI in this set as a prefix may be assumed to be in the same protection space.";
	rdfs:domain calli:Realm.

calli:forbidden a owl:ObjectProperty;
	rdfs:comment "The RDFa template used when an agent is forbidden from the requested resource.";
	rdfs:domain calli:Realm;
	rdfs:range calli:Template.

calli:unauthorized a owl:ObjectProperty;
	rdfs:comment "The RDFa template used when an agent is aunothorized from the requested resource.";
	rdfs:domain calli:Realm;
	rdfs:range calli:Template.

calli:scribe a owl:ObjectProperty;
	rdfs:comment "Credential or group of credentials that can copy this resource remotely.";
	rdfs:domain calli:Copyable;
	rdfs:range calli:Party.

calli:curator a owl:ObjectProperty;
	rdfs:comment "Credential or group of credentials that will maintain any copied resources.";
	rdfs:domain calli:Copyable;
	rdfs:range calli:Party.

calli:maintainer a owl:ObjectProperty;
	rdfs:comment "Credential or group of credentials that can interact with this resource remotely.";
	rdfs:range calli:Party.

calli:member a owl:ObjectProperty;
	rdfs:comment "Credential that is part of this group.";
	rdfs:domain calli:Group;
	rdfs:range calli:Credential.

calli:soundex a owl:DatatypeProperty;
	rdfs:comment "A soundex encoding of one of this resource's label or label prefix.";
	rdfs:range xsd:string.

calli:copyOf a owl:ObjectProperty, owl:FunctionalProperty;
	rdfs:comment "The authoritative canonical URL of which this alias is a copy of.";
	rdfs:domain calli:Alias.

calli:aliasOf a owl:ObjectProperty, owl:FunctionalProperty;
	rdfs:comment "The canonical URL for this alias.";
	rdfs:domain calli:Alias.

calli:minified a owl:DatatypeProperty, owl:FunctionalProperty;
	rdfs:comment "Level of minification that should be applied to this bundle. Zero represents no minification. One represents minimal minification.";
	rdfs:domain calli:ScriptBundle;
	rdfs:range xsd:integer.

################################
# Thing
################################

calli:nobody a calli:NobodyRealm.

