# 
#    Portions Copyright (c) 2009-10 Zepheira LLC, Some Rights Reserved
#    Portions Copyright (c) 2010-11 Talis Inc, Some Rights Reserved
#    Portions Copyright (c) 2011-2012 3 Round Stones Inc, Some Rights Reserved
# 
#    Licensed under the Apache License, Version 2.0 (the "License");
#    you may not use this file except in compliance with the License.
#    You may obtain a copy of the License at
# 
#        http://www.apache.org/licenses/LICENSE-2.0
# 
#    Unless required by applicable law or agreed to in writing, software
#    distributed under the License is distributed on an "AS IS" BASIS,
#    WITHOUT WARRANTIES OR CONDITIONS OF ANY KIND, either express or implied.
#    See the License for the specific language governing permissions and
#    limitations under the License.
#
@prefix xsd:<http://www.w3.org/2001/XMLSchema#>.
@prefix rdf:<http://www.w3.org/1999/02/22-rdf-syntax-ns#>.
@prefix rdfs:<http://www.w3.org/2000/01/rdf-schema#>.
@prefix owl:<http://www.w3.org/2002/07/owl#>.
@prefix sd:<http://www.w3.org/ns/sparql-service-description#>.
@prefix foaf:<http://xmlns.com/foaf/0.1/>.
@prefix calli:<http://callimachusproject.org/rdf/2009/framework#>.

<> a <types/RdfSchemaGraph>;
    foaf:primaryTopic <http://callimachusproject.org/rdf/2009/framework>.

################################
# Ontology
################################

<http://callimachusproject.org/rdf/2009/framework> a owl:Ontology;
    rdfs:label "Callimachus Ontology";
    rdfs:comment "Vocabulary used to create Callimachus applications";
    owl:versionInfo "1.4".

################################
# Class
################################

calli:Purl a owl:Class;
    rdfs:label "PURL";
    rdfs:comment "Persistent Uniform Resource Location of a Web resource";
    rdfs:isDefinedBy <http://callimachusproject.org/rdf/2009/framework>.

calli:Composite a owl:Class;
    rdfs:label "Composite";
    rdfs:comment "Class of resources that contain nested components, where the component URIs have their parent URI as a prefix";
    rdfs:isDefinedBy <http://callimachusproject.org/rdf/2009/framework>.

calli:Folder a owl:Class;
    rdfs:subClassOf calli:Composite, calli:Purl;
    rdfs:label "Folder";
    rdfs:comment "A resource URI namespace ending in a slash";
    rdfs:isDefinedBy <http://callimachusproject.org/rdf/2009/framework>.

calli:Realm a owl:Class;
    rdfs:subClassOf calli:Folder;
    rdfs:label "Realm";
    rdfs:comment "Web application realm";
    rdfs:isDefinedBy <http://callimachusproject.org/rdf/2009/framework>.

calli:Origin a owl:Class;
    rdfs:subClassOf calli:Realm;
    rdfs:label "Origin";
    rdfs:comment "A URI with a '/' path that is served by a Callimachus system";
    rdfs:isDefinedBy <http://callimachusproject.org/rdf/2009/framework>.

calli:Credential a owl:Class;
    rdfs:label "Credential";
    rdfs:comment "Client Web credential";
    rdfs:isDefinedBy <http://callimachusproject.org/rdf/2009/framework>.

calli:AuthenticationManager a owl:Class;
    rdfs:label "Authentication Manager";
    rdfs:comment "A managed set of users that can authenticate using HTTP digest credentials";
    rdfs:isDefinedBy <http://callimachusproject.org/rdf/2009/framework>.

calli:DigestManager a owl:Class;
    rdfs:subClassOf calli:AuthenticationManager;
    rdfs:label "Digest Manager";
    rdfs:comment "A managed set of users that can authenticate using HTTP digest credentials";
    rdfs:isDefinedBy <http://callimachusproject.org/rdf/2009/framework>.

calli:OpenIDManager a owl:Class;
    rdfs:subClassOf calli:AuthenticationManager;
    rdfs:label "OpenID Manager";
    rdfs:comment "Login manager for a particular OpenID provider";
    rdfs:isDefinedBy <http://callimachusproject.org/rdf/2009/framework>.

calli:FacebookManager a owl:Class;
    rdfs:subClassOf calli:AuthenticationManager;
    rdfs:label "Facebook Manager";
    rdfs:comment "Login manager for a Facebook app";
    rdfs:isDefinedBy <http://callimachusproject.org/rdf/2009/framework>.

calli:Party a owl:Class;
    rdfs:label "Party";
    rdfs:comment "A user or group of users";
    rdfs:isDefinedBy <http://callimachusproject.org/rdf/2009/framework>.

calli:User a owl:Class;
    rdfs:subClassOf calli:Party;
    rdfs:label "Agent";
    rdfs:comment "A user account";
    rdfs:isDefinedBy <http://callimachusproject.org/rdf/2009/framework>.

calli:Group a owl:Class;
    rdfs:subClassOf calli:Party;
    rdfs:label "Group";
    rdfs:comment "A collection of users";
    rdfs:isDefinedBy <http://callimachusproject.org/rdf/2009/framework>.

calli:Domain a owl:Class;
    rdfs:subClassOf calli:Party;
    rdfs:label "Domain";
    rdfs:comment "A collection of network domains";
    rdfs:isDefinedBy <http://callimachusproject.org/rdf/2009/framework>.

calli:ScriptBundle a owl:Class;
    rdfs:label "Script Bundle";
    rdfs:comment "A collection of JavaScript files that are downloaded and compressed together";
    rdfs:isDefinedBy <http://callimachusproject.org/rdf/2009/framework>.

calli:Page a owl:Class;
    rdfs:subClassOf foaf:Document;
    rdfs:label "Page";
    rdfs:comment "A Callimachus XHTML page";
    rdfs:isDefinedBy <http://callimachusproject.org/rdf/2009/framework>.

calli:Markdown a owl:Class;
    rdfs:subClassOf foaf:Document;
    rdfs:label "Markdown";
    rdfs:comment "A Callimachus Markdown document";
    rdfs:isDefinedBy <http://callimachusproject.org/rdf/2009/framework>.

calli:Pipeline a owl:Class;
    rdfs:subClassOf foaf:Document;
    rdfs:label "Pipeline";
    rdfs:comment "A Callimachus XProc file";
    rdfs:isDefinedBy <http://callimachusproject.org/rdf/2009/framework>.

calli:XQuery a owl:Class;
    rdfs:subClassOf foaf:Document;
    rdfs:label "XQuery";
    rdfs:comment "A Callimachus XQuery file";
    rdfs:isDefinedBy <http://callimachusproject.org/rdf/2009/framework>.

calli:XslTransform a owl:Class;
    rdfs:subClassOf foaf:Document;
    rdfs:label "XSL Transform";
    rdfs:comment "A Callimachus XSL file";
    rdfs:isDefinedBy <http://callimachusproject.org/rdf/2009/framework>.

calli:RdfDatasource a owl:Class;
    rdfs:subClassOf sd:Service;
    rdfs:label "RDF Datasource";
    rdfs:comment "An RDF source";
    rdfs:isDefinedBy <http://callimachusproject.org/rdf/2009/framework>.

calli:SqlDatasource a owl:Class;
    rdfs:label "SQL Datasource";
    rdfs:comment "JDBC database connection information";
    rdfs:isDefinedBy <http://callimachusproject.org/rdf/2009/framework>.

calli:ZipArchive a owl:Class;
    rdfs:subClassOf foaf:Document;
    rdfs:label "ZIP Archive";
    rdfs:comment "ZIP archive files";
    rdfs:isDefinedBy <http://callimachusproject.org/rdf/2009/framework>.

################################
# Annotation
################################

calli:reader a owl:AnnotationProperty;
    rdfs:label "reader";
    rdfs:comment "User or group that can view this resource and individual resources of this class";
    rdfs:isDefinedBy <http://callimachusproject.org/rdf/2009/framework>.

calli:subscriber a owl:AnnotationProperty;
    rdfs:subPropertyOf calli:reader;
    rdfs:label "subscribe";
    rdfs:comment "User or group that can read comments and write comments for this resource and resources of this class";
    rdfs:isDefinedBy <http://callimachusproject.org/rdf/2009/framework>.

calli:author a owl:AnnotationProperty;
    rdfs:label "author";
    rdfs:comment "User or group that can create an instance resource of this class";
    rdfs:isDefinedBy <http://callimachusproject.org/rdf/2009/framework>.

calli:contributor a owl:AnnotationProperty;
    rdfs:subPropertyOf calli:subscriber;
    rdfs:label "contributor";
    rdfs:comment "User or group that can create a resource in this namespace";
    rdfs:isDefinedBy <http://callimachusproject.org/rdf/2009/framework>.

calli:editor a owl:AnnotationProperty;
    rdfs:subPropertyOf calli:contributor, calli:author;
    rdfs:label "editor";
    rdfs:comment "User or group that can create resources in this namespace, can edit this resource, and edit members of this class";
    rdfs:isDefinedBy <http://callimachusproject.org/rdf/2009/framework>.

calli:administrator a owl:AnnotationProperty;
    rdfs:subPropertyOf calli:editor;
    rdfs:label "administrator";
    rdfs:comment "User or group that can interact, create and modify this resource and members of this class";
    rdfs:isDefinedBy <http://callimachusproject.org/rdf/2009/framework>.

calli:edit a owl:AnnotationProperty;
    rdfs:label "edit";
    rdfs:comment "The RDFa page template used to edit individual resources of this class using a Web browser";
    rdfs:isDefinedBy <http://callimachusproject.org/rdf/2009/framework>.

calli:view a owl:AnnotationProperty;
    rdfs:label "view";
    rdfs:comment "The RDFa page template used to display individual resources of this class in a Web browser";
    rdfs:isDefinedBy <http://callimachusproject.org/rdf/2009/framework>.

calli:create a owl:AnnotationProperty;
    rdfs:label "create";
    rdfs:comment "The RDFa page template used to create resources of this class using a Web browser";
    rdfs:isDefinedBy <http://callimachusproject.org/rdf/2009/framework>.

calli:documentTag a owl:AnnotationProperty;
    rdfs:label "document tag";
    rdfs:comment "IRI of a tag name for an XML document element of resources of this class";
    rdfs:isDefinedBy <http://callimachusproject.org/rdf/2009/framework>.

calli:mediaType a owl:AnnotationProperty;
    rdfs:label "media type";
    rdfs:comment "The content media type for binary or text representations of resources of this class";
    rdfs:isDefinedBy <http://callimachusproject.org/rdf/2009/framework>.

calli:icon a owl:AnnotationProperty;
    rdfs:label "icon";
    rdfs:comment "A 16x16 px Portable Network Graphic representing a single resource of this class";
    rdfs:isDefinedBy <http://callimachusproject.org/rdf/2009/framework>.

calli:thumbnail a owl:AnnotationProperty;
    rdfs:label "thumbnail";
    rdfs:comment "A 256x256 px Scalable Vector Graphic representing a single resource of this class";
    rdfs:isDefinedBy <http://callimachusproject.org/rdf/2009/framework>.

calli:type a owl:AnnotationProperty;
    rdfs:label "type";
    rdfs:comment "The content type for binary or text representations of objects for this property, or msg:object for this message class";
    rdfs:isDefinedBy <http://callimachusproject.org/rdf/2009/framework>.

calli:expect a owl:AnnotationProperty;
    rdfs:label "expect";
    rdfs:comment "Placed on a method to indicate the HTTP response status code of a successful response. Possible values include '201-created', '202-accepted', '205-reset-content', '300-multiple-choices', '301-moved-permanently', and '302-found'";
    rdfs:isDefinedBy <http://callimachusproject.org/rdf/2009/framework>.

calli:header a owl:AnnotationProperty;
    rdfs:label "header";
    rdfs:comment "Placed on message parameters that should be populated with request headers. Placed on messages to add a response header. Response header of 'cache-control:no-validate' disable server side validation and 'cache-control:cache-range' use strong etag validation";
    rdfs:isDefinedBy <http://callimachusproject.org/rdf/2009/framework>.

calli:method a owl:AnnotationProperty;
    rdfs:label "method";
    rdfs:comment "Placed on messages that should be called for the given HTTP method";
    rdfs:isDefinedBy <http://callimachusproject.org/rdf/2009/framework>.

calli:query a owl:AnnotationProperty;
    rdfs:label "query";
    rdfs:comment "Placed on messages that should be called when the given request query parameter name is sent without a value. Placed on message properties that should be populated with request GET query parameters";
    rdfs:isDefinedBy <http://callimachusproject.org/rdf/2009/framework>.

calli:requires a owl:AnnotationProperty;
    rdfs:label "requires";
    rdfs:comment "The role required to be capable of successfully requesting a message of this class";
    rdfs:isDefinedBy <http://callimachusproject.org/rdf/2009/framework>.

calli:rel a owl:AnnotationProperty;
    rdfs:label "rel";
    rdfs:comment "Placed on properties or messages and describes the relationship between the message target and message response";
    rdfs:isDefinedBy <http://callimachusproject.org/rdf/2009/framework>.

calli:title a owl:AnnotationProperty;
    rdfs:label "title";
    rdfs:comment "Labels the relationship between message target and message response such that it can be used as identification within a human-readable menu";
    rdfs:isDefinedBy <http://callimachusproject.org/rdf/2009/framework>.

calli:transform a owl:DeprecatedProperty, owl:AnnotationProperty;
    rdfs:label "transform";
    rdfs:comment "The messages that should be used to transform the parameter or response";
    rdfs:isDefinedBy <http://callimachusproject.org/rdf/2009/framework>.

calli:copy a owl:AnnotationProperty;
    rdfs:label "get";
    rdfs:comment "This request handler should return the GET response of the given template URL";
    rdfs:isDefinedBy <http://callimachusproject.org/rdf/2009/framework>.

calli:post a owl:AnnotationProperty;
    rdfs:label "post";
    rdfs:comment "This request handler should delegate a POST request to the given template URL";
    rdfs:isDefinedBy <http://callimachusproject.org/rdf/2009/framework>.

calli:put a owl:AnnotationProperty;
    rdfs:label "put";
    rdfs:comment "This request handler should delegate a PUT request to the given template URL";
    rdfs:isDefinedBy <http://callimachusproject.org/rdf/2009/framework>.

calli:patch a owl:AnnotationProperty;
    rdfs:label "patch";
    rdfs:comment "This request handler should delegate a PATCH request to the given template URL";
    rdfs:isDefinedBy <http://callimachusproject.org/rdf/2009/framework>.

calli:delete a owl:AnnotationProperty;
    rdfs:label "delete";
    rdfs:comment "This request handler should delegate a DELETE request to the given template URL";
    rdfs:isDefinedBy <http://callimachusproject.org/rdf/2009/framework>.

calli:canonical a owl:AnnotationProperty;
    rdfs:label "canonical";
    rdfs:comment "Target template URI that this request handler (301) redirects to";
    rdfs:isDefinedBy <http://callimachusproject.org/rdf/2009/framework>.

calli:alternate a owl:AnnotationProperty;
    rdfs:label "alternate";
    rdfs:comment "Target template URI that this request handler (302) redirects to";
    rdfs:isDefinedBy <http://callimachusproject.org/rdf/2009/framework>.

calli:describedby a owl:AnnotationProperty;
    rdfs:label "describedby";
    rdfs:comment "Target template URI that this request handler (303) redirects to";
    rdfs:isDefinedBy <http://callimachusproject.org/rdf/2009/framework>.

calli:resides a owl:AnnotationProperty;
    rdfs:label "resides";
    rdfs:comment "Target template URI that this request handler (307) redirects to";
    rdfs:isDefinedBy <http://callimachusproject.org/rdf/2009/framework>.

calli:moved a owl:AnnotationProperty;
    rdfs:label "moved";
    rdfs:comment "Target template URI that this request handler (308) redirects to";
    rdfs:isDefinedBy <http://callimachusproject.org/rdf/2009/framework>.

calli:missing a owl:AnnotationProperty;
    rdfs:label "missing";
    rdfs:comment "Document describing that this resource is disabled or missing";
    rdfs:isDefinedBy <http://callimachusproject.org/rdf/2009/framework>.

calli:gone a owl:AnnotationProperty;
    rdfs:label "gone";
    rdfs:comment "Document describing that this resource is gone";
    rdfs:isDefinedBy <http://callimachusproject.org/rdf/2009/framework>.

################################
# Property
################################

calli:authority a owl:FunctionalProperty, owl:DatatypeProperty;
    rdfs:label "authority";
    rdfs:comment "An hostname, possiblely followed by a colon and port";
    rdfs:domain calli:Credential;
    rdfs:range rdf:PlainLiteral;
    rdfs:isDefinedBy <http://callimachusproject.org/rdf/2009/framework>.

calli:username a owl:FunctionalProperty, owl:DatatypeProperty;
    rdfs:label "username";
    rdfs:comment "The username to login using";
    rdfs:domain calli:Credential;
    rdfs:range rdf:PlainLiteral;
    rdfs:isDefinedBy <http://callimachusproject.org/rdf/2009/framework>.

calli:passwordFile a owl:FunctionalProperty, owl:OjectProperty;
    rdfs:label "password file";
    rdfs:comment "Location of a text file containing the password in BASE64";
    rdfs:domain calli:Credential;
    rdfs:range foaf:Document;
    rdfs:isDefinedBy <http://callimachusproject.org/rdf/2009/framework>.

calli:passwordDigest a owl:ObjectProperty;
    rdfs:label "password digest";
    rdfs:comment "A document of the MD5 sum of email:authName:password in HEX encoding";
    rdfs:domain calli:User;
    rdfs:range foaf:Document;
    rdfs:isDefinedBy <http://callimachusproject.org/rdf/2009/framework>.

calli:name a owl:DatatypeProperty, owl:FunctionalProperty;
    rdfs:label "name";
    rdfs:comment "The username for this agent";
    rdfs:domain calli:User;
    rdfs:range rdf:PlainLiteral;
    rdfs:isDefinedBy <http://callimachusproject.org/rdf/2009/framework>.

calli:email a owl:DatatypeProperty, owl:FunctionalProperty;
    rdfs:label "email";
    rdfs:comment "The primary email address for this user";
    rdfs:domain calli:User;
    rdfs:range rdf:PlainLiteral;
    rdfs:isDefinedBy <http://callimachusproject.org/rdf/2009/framework>.

calli:authButton a owl:FunctionalProperty, owl:ObjectProperty;
    rdfs:label "auth button";
    rdfs:comment "Branded authentication images to initiate logins";
    rdfs:domain calli:AuthenticationManager;
    rdfs:range foaf:Image;
    rdfs:isDefinedBy <http://callimachusproject.org/rdf/2009/framework>.

calli:authNamespace a owl:FunctionalProperty, owl:ObjectProperty;
    rdfs:label "auth namespace";
    rdfs:comment "Folder of users that can be authenticated by this realm";
    rdfs:domain calli:DigestManager;
    rdfs:range calli:Folder;
    rdfs:isDefinedBy <http://callimachusproject.org/rdf/2009/framework>.

calli:authName a owl:FunctionalProperty, owl:DatatypeProperty;
    rdfs:label "auth name";
    rdfs:comment "A string to be displayed to users so they know which username and password to use. This string should contain at least the name of the host performing the authentication and might additionally indicate the collection of users who might have access. This string is used to encode the passwords and changing it will invalidates existing encoded passwords";
    rdfs:domain calli:DigestManager;
    rdfs:isDefinedBy <http://callimachusproject.org/rdf/2009/framework>.

calli:openIdEndpointUrl a owl:FunctionalProperty, owl:DatatypeProperty;
    rdfs:label "openID endpoint URL";
	rdfs:comment "OpenID provider URL";
	rdfs:domain calli:OpenIDManager;
	rdfs:range xsd:string;
    rdfs:isDefinedBy <http://callimachusproject.org/rdf/2009/framework>.

calli:openIdRealm a owl:FunctionalProperty, owl:DatatypeProperty;
	rdfs:label "openID realm";
	rdfs:comment "OpenID realm pattern. It MUST NOT contain a URI fragment and MAY contain a wild-card at the beginning of the URL authority section. A wild-card consists of the characters '*.' prepended to the DNS name in the authority section of the URL.";
	rdfs:domain calli:OpenIDManager;
	rdfs:range xsd:string;
    rdfs:isDefinedBy <http://callimachusproject.org/rdf/2009/framework>.

calli:facebookAppId a owl:FunctionalProperty, owl:DatatypeProperty;
    rdfs:label "facebook App ID";
    rdfs:comment "The app ID as provided by facebook";
    rdfs:domain calli:FacebookManager;
    rdfs:isDefinedBy <http://callimachusproject.org/rdf/2009/framework>.

calli:facebookSecret a owl:FunctionalProperty, owl:ObjectProperty;
    rdfs:label "facebook secret";
    rdfs:comment "The URI of an app secret as provided by facebook";
    rdfs:domain calli:FacebookManager;
    rdfs:isDefinedBy <http://callimachusproject.org/rdf/2009/framework>.

calli:secret a owl:FunctionalProperty, owl:ObjectProperty;
    rdfs:label "secret";
    rdfs:comment "A document of random bits in Base 64 encoding";
    rdfs:domain calli:Origin;
    rdfs:range foaf:Document;
    rdfs:isDefinedBy <http://callimachusproject.org/rdf/2009/framework>.

calli:credentials a owl:ObjectProperty;
    rdfs:label "credentials";
    rdfs:comment "Credentials that can be used by resources hosted in this realm";
    rdfs:domain calli:Realm;
    rdfs:range calli:Credential;
    rdfs:isDefinedBy <http://callimachusproject.org/rdf/2009/framework>.

calli:error a owl:ObjectProperty;
    rdfs:label "error";
    rdfs:comment "An XPROC pipeline file that should be used to transform/style simple error pages";
    rdfs:domain calli:Realm;
    rdfs:range calli:Purl;
    rdfs:isDefinedBy <http://callimachusproject.org/rdf/2009/framework>.

calli:forbidden a owl:ObjectProperty;
    rdfs:label "forbidden";
    rdfs:comment "The XHTML page template used when an agent is forbidden from the requested resource";
    rdfs:domain calli:Realm;
    rdfs:range calli:Purl;
    rdfs:isDefinedBy <http://callimachusproject.org/rdf/2009/framework>.

calli:unauthorized a owl:ObjectProperty;
    rdfs:label "authorized";
    rdfs:comment "The XHTML page used when an agent is aunothorized from the requested resource";
    rdfs:domain calli:Realm;
    rdfs:range calli:Purl;
    rdfs:isDefinedBy <http://callimachusproject.org/rdf/2009/framework>.

calli:authentication a owl:ObjectProperty;
    rdfs:label "authentication";
    rdfs:comment "The realm used for authentication";
    rdfs:domain calli:Realm;
    rdfs:range calli:AuthenticationManager;
    rdfs:isDefinedBy <http://callimachusproject.org/rdf/2009/framework>.

calli:member a owl:ObjectProperty;
    rdfs:label "member";
    rdfs:comment "Agent that is part of this group";
    rdfs:domain calli:Group;
    rdfs:range calli:Agent;
    rdfs:isDefinedBy <http://callimachusproject.org/rdf/2009/framework>.

calli:anonymousFrom a owl:DatatypeProperty;
    rdfs:label "anonymous from";
    rdfs:comment "Domain Name System suffix of agents that are permitted anonymous access to the resources associated with this domain";
    rdfs:domain calli:Domain;
    rdfs:range xsd:string;
    rdfs:isDefinedBy <http://callimachusproject.org/rdf/2009/framework>.

calli:everyoneFrom a owl:DatatypeProperty;
    rdfs:label "everyone from";
    rdfs:comment "Domain Name System suffix of authenticated agents that are permitted to the resources associated with this domain";
    rdfs:domain calli:Domain;
    rdfs:range xsd:string;
    rdfs:isDefinedBy <http://callimachusproject.org/rdf/2009/framework>.

calli:nobodyFrom a owl:DatatypeProperty;
    rdfs:label "nobody from";
    rdfs:comment "Domain Name System suffix of agents that are not permitted in this domain";
    rdfs:domain calli:Domain;
    rdfs:range xsd:string;
    rdfs:isDefinedBy <http://callimachusproject.org/rdf/2009/framework>.

calli:cacheControl a owl:DatatypeProperty;
    rdfs:label "cache-control";
    rdfs:comment "A response Cache-Control directive";
    rdfs:domain calli:Purl;
    rdfs:range xsd:string;
    rdfs:isDefinedBy <http://callimachusproject.org/rdf/2009/framework>.

calli:hasComponent a owl:ObjectProperty;
    rdfs:subPropertyOf rdfs:member;
    rdfs:label "has component";
    rdfs:comment "A nested resource with a URI that starts with this resource URI with one additional path, fragement, or component segment";
    rdfs:domain calli:Composite;
    rdfs:isDefinedBy <http://callimachusproject.org/rdf/2009/framework>.

calli:minified a owl:DatatypeProperty;
    rdfs:label "minified";
    rdfs:comment "Level of minification that should be applied to this bundle. Zero represents no minification. One represents minimal minification";
    rdfs:domain calli:ScriptBundle;
    rdfs:range xsd:integer;
    rdfs:isDefinedBy <http://callimachusproject.org/rdf/2009/framework>.

calli:allowOrigin a owl:DatatypeProperty;
    rdfs:label "allow origin";
    rdfs:comment "An HTTP code origin that is permitted to authenticate and access protected resources by behave of the requesting agent";
    rdfs:domain calli:Realm;
    rdfs:range xsd:string;
    rdfs:isDefinedBy <http://callimachusproject.org/rdf/2009/framework>.

calli:layout a owl:FunctionalProperty, owl:ObjectProperty;
    rdfs:label "layout";
    rdfs:comment "An XQuery transform to add header/footer markup to page templates";
    rdfs:domain calli:Realm;
    rdfs:isDefinedBy <http://callimachusproject.org/rdf/2009/framework>.

calli:jdbcUrl a owl:FunctionalProperty, owl:DatatypeProperty;
    rdfs:label "jdbc url";
    rdfs:comment "The JDBC connection url for connecting to the database";
    rdfs:domain calli:SqlDatasource;
    rdfs:range xsd:string;
    rdfs:isDefinedBy <http://callimachusproject.org/rdf/2009/framework>.

calli:driverClassName a owl:DatatypeProperty;
    rdfs:label "driver class name";
    rdfs:comment "Java class name of the driver that should be used";
    rdfs:domain calli:SqlDatasource;
    rdfs:range xsd:string;
    rdfs:isDefinedBy <http://callimachusproject.org/rdf/2009/framework>.

calli:driverJar a owl:ObjectProperty;
    rdfs:label "driver jar";
    rdfs:comment "JAR that contains the driver class or one of its dependencies";
    rdfs:domain calli:SqlDatasource;
    rdfs:isDefinedBy <http://callimachusproject.org/rdf/2009/framework>.

calli:maxActive a owl:FunctionalProperty, owl:DatatypeProperty;
    rdfs:label "max idle";
    rdfs:comment "Maximum number of database connections in pool";
    rdfs:domain calli:SqlDatasource;
    rdfs:range xsd:integer;
    rdfs:isDefinedBy <http://callimachusproject.org/rdf/2009/framework>.

calli:maxIdle a owl:FunctionalProperty, owl:DatatypeProperty;
    rdfs:label "max idle";
    rdfs:comment "Maximum number of idle database connections to retain in pool";
    rdfs:domain calli:SqlDatasource;
    rdfs:range xsd:integer;
    rdfs:isDefinedBy <http://callimachusproject.org/rdf/2009/framework>.

calli:maxWait a owl:FunctionalProperty, owl:DatatypeProperty;
    rdfs:label "max wait";
    rdfs:comment "Maximum time to wait for a database connection to become available in ms";
    rdfs:domain calli:SqlDatasource;
    rdfs:range xsd:integer;
    rdfs:isDefinedBy <http://callimachusproject.org/rdf/2009/framework>.

calli:validationQuery a owl:FunctionalProperty, owl:DatatypeProperty;
    rdfs:label "validation query";
    rdfs:comment "SQL SELECT query to validate connections";
    rdfs:domain calli:SqlDatasource;
    rdfs:range xsd:string;
    rdfs:isDefinedBy <http://callimachusproject.org/rdf/2009/framework>.

